specs/Spec.Agile.HMAC.fst
@@ -1,4 +1,4 @@
-module Spec.HMAC
+module Spec.Agile.HMAC
 
 module S = Lib.Sequence
 
@@ -8,7 +8,7 @@ open Lib.IntTypes
 
 let wrap (a:hash_alg) (key: bytes{Seq.length key <= max_input_length a}): Tot (lbytes (block_length a))
 =
-  let key0 = if Seq.length key <= block_length a then key else Spec.Hash.hash a key in
+  let key0 = if Seq.length key <= block_length a then key else Spec.Agile.Hash.hash a key in
   let paddingLength = block_length a - Seq.length key0 in
   Seq.append key0 (Seq.create paddingLength (u8 0))
 
@@ -31,6 +31,6 @@ let hmac a key data =
   assert_norm (pow2 32 < pow2 61);
   assert_norm (pow2 32 < pow2 125);
   let k = wrap a key in
-  let h1 = Spec.Hash.hash a (Seq.append (xor (u8 0x36) k) data) in
-  let h2 = Spec.Hash.hash a (Seq.append (xor (u8 0x5c) k) h1) in
+  let h1 = Spec.Agile.Hash.hash a (Seq.append (xor (u8 0x36) k) data) in
+  let h2 = Spec.Agile.Hash.hash a (Seq.append (xor (u8 0x5c) k) h1) in
   h2
