providers/evercrypt/EverCrypt.Hash.fsti
@@ -216,7 +216,7 @@ val init: #a:e_alg -> (
   (requires invariant s)
   (ensures fun h0 _ h1 ->
     invariant s h1 /\
-    repr s h1 == Spec.Hash.init a /\
+    repr s h1 == Spec.Agile.Hash.init a /\
     M.(modifies (footprint s h0) h0 h1) /\
     footprint s h0 == footprint s h1 /\
     preserves_freeable s h0 h1))
@@ -246,7 +246,7 @@ val update:
     M.(modifies (footprint s h0) h0 h1) /\
     footprint s h0 == footprint s h1 /\
     invariant s h1 /\
-    repr s h1 == Spec.Hash.update a (repr s h0) (B.as_seq h0 block) /\
+    repr s h1 == Spec.Agile.Hash.update a (repr s h0) (B.as_seq h0 block) /\
     preserves_freeable s h0 h1))
 
 // Note that we pass the data length in bytes (rather than blocks).
@@ -267,7 +267,7 @@ val update_multi:
     M.(modifies (footprint s h0) h0 h1) /\
     footprint s h0 == footprint s h1 /\
     invariant s h1 /\
-    repr s h1 == Spec.Hash.update_multi a (repr s h0) (B.as_seq h0 blocks) /\
+    repr s h1 == Spec.Agile.Hash.update_multi a (repr s h0) (B.as_seq h0 blocks) /\
     preserves_freeable s h0 h1))
 
 val update_last_256: Hacl.Hash.Definitions.update_last_st SHA2_256
@@ -302,7 +302,7 @@ val update_last:
     invariant s h1 /\
     (B.length last + Seq.length (Spec.Hash.PadFinish.pad a (v total_len))) % block_length a = 0 /\
     repr s h1 ==
-      Spec.Hash.update_multi a (repr s h0)
+      Spec.Agile.Hash.update_multi a (repr s h0)
         (Seq.append (B.as_seq h0 last) (Spec.Hash.PadFinish.pad a (v total_len))) /\
     M.(modifies (footprint s h0) h0 h1) /\
     footprint s h0 == footprint s h1 /\
@@ -375,4 +375,4 @@ val hash:
     M.(loc_disjoint (loc_buffer input) (loc_buffer dst)))
   (ensures fun h0 _ h1 ->
     M.(modifies (loc_buffer dst) h0 h1) /\
-    B.as_seq h1 dst == Spec.Hash.hash a (B.as_seq h0 input))
+    B.as_seq h1 dst == Spec.Agile.Hash.hash a (B.as_seq h0 input))
