providers/evercrypt/fst/EverCrypt.HKDF.fst
@@ -17,8 +17,8 @@ open FStar.Integers
 open EverCrypt.Hash
 
 open Spec.Hash.Definitions
-open Spec.HKDF
-friend Spec.HKDF
+open Spec.Agile.HKDF
+friend Spec.Agile.HKDF
 
 friend Lib.IntTypes
 
@@ -35,7 +35,7 @@ val hkdf_expand_loop:
   len     : UInt32.t { UInt32.v len == B.length okm } ->
   hashed  : B.buffer Lib.IntTypes.uint8 { B.length hashed == Spec.Hash.Definitions.hash_length a + v infolen + 1} ->
   i       : UInt8.t {
-    Spec.HMAC.keysized a (length prk) /\
+    Spec.Agile.HMAC.keysized a (length prk) /\
     disjoint okm prk /\
     disjoint hashed okm /\
     disjoint hashed prk /\
@@ -86,7 +86,7 @@ let rec hkdf_expand_loop a okm prk prklen infolen len hashed i =
       // Seq.lemma_eq_intro (as_seq h1 counter) ctr1;
       // assert(tag2 == HMAC.hmac a v_prk (as_seq h1 hashed1));
       Seq.lemma_eq_intro (as_seq h1 info_counter) text;
-      assert(tag2 == Spec.HMAC.hmac a prk text)  ))
+      assert(tag2 == Spec.Agile.HMAC.hmac a prk text)  ))
   else (
     HMAC.compute a tag prk prklen hashed (tlen + infolen + 1ul);
     ( let h2 = ST.get() in
@@ -98,7 +98,7 @@ let rec hkdf_expand_loop a okm prk prklen infolen len hashed i =
       let text = tag1 @| info @| ctr1 in
       // assert(tag2 == HMAC.hmac (Ghost.hide a) prk (as_seq h1 hashed));
       Seq.lemma_eq_intro (as_seq h1 hashed) text ;
-      assert(tag2 == Spec.HMAC.hmac a prk text )));
+      assert(tag2 == Spec.Agile.HMAC.hmac a prk text )));
 
   // copy it to the result; iterate if required
   let h2 = ST.get() in
